Add FiniteAddresses.

src/mem/Addresses/FiniteAddresses.v
@@ -4,7 +4,8 @@ From Coq Require Import
 
 From Vellvm Require Import
   Numeric.Coqlib
-  Utils.Error.
+  Utils.Error
+  Utils.Tactics.
 
 From Mem Require Import
   Addresses.MemoryAddress
@@ -60,10 +61,10 @@ Module FinAddrType <: CORE_ADDRESS.
 End FinAddrType.
 
 Module FinNull <: HAS_NULL FinAddrType.
-  Definition null := (Int64.zero, nil_prov)%Z.
+  Definition null := (repr 0, nil_prov)%Z.
 
-  Definition is_null (a : FinAddrType.t) :=
-    Int64.eq (fst null) (fst a).
+  Definition is_null (a : FinAddrType.t) : bool :=
+    Integers.eq (fst null) (fst a).
 
   Lemma null_is_null :
     is_null null = true.
@@ -73,7 +74,7 @@ Module FinNull <: HAS_NULL FinAddrType.
 End FinNull.
 
 Module FinPTOI <: HAS_PTOI FinAddrType.
-  Definition ptr_to_int := fun (ptr : FinAddrType.t) => Int64.unsigned (fst ptr).
+  Definition ptr_to_int := fun (ptr : FinAddrType.t) => @Integers.unsigned 64 (fst ptr).
 End FinPTOI.
 
 Module Type Fin_HAS_POINTER_ARITHMETIC_CORE <: HAS_POINTER_ARITHMETIC_CORE FinAddrType.
@@ -83,10 +84,10 @@ Module Type Fin_HAS_POINTER_ARITHMETIC_CORE <: HAS_POINTER_ARITHMETIC_CORE FinAd
   Definition ptr_add (a : FinAddrType.t) (i : Z) : err FinAddrType.t
     := match a with
        | (ptr, pr) =>
-           let res := Int64.unsigned ptr + i in
-           if (res >? Int64.max_unsigned) || (res <? 0)
-           then inl "ptr_add: out of bounds."%string
-           else ret (Int64.repr res, pr)
+           let res := @Integers.unsigned 64 ptr + i in
+           if (res <? 0)%Z || (res >=? @Integers.modulus 64)%Z
+           then inl ("ptr_add: out of range (" ++ show i ++ ").")%string
+           else ret (@Integers.repr 64 res, pr)
        end.
 
   Lemma ptr_add_0 :
@@ -97,353 +98,108 @@ Module Type Fin_HAS_POINTER_ARITHMETIC_CORE <: HAS_POINTER_ARITHMETIC_CORE FinAd
     unfold ptr_add.
     destruct ptr.
     rewrite Z.add_0_r in *.
-    destruct ((Int64.unsigned i >? Int64.max_unsigned) || (Int64.unsigned i <? 0)) eqn:bounds.
-    - (* Contradiction *)
-      exfalso.
-      pose proof Int64.unsigned_range_2 i.
-      lia.
-    - setoid_rewrite Int64.repr_unsigned.
-      reflexivity.
+    pose proof Integers.unsigned_range i.
+    break_match; try lia.
+    rewrite Integers.repr_unsigned.
+    reflexivity.
   Qed.
 End Fin_HAS_POINTER_ARITHMETIC_CORE.
 
-Module FinPROV <: PROVENANCE(FinAddr)
-with Definition Prov := Prov
-with Definition address_provenance
-    := fun (a : FinAddr.addr) => snd a
-with Definition Provenance := Provenance
-with Definition AllocationId := AllocationId
-with Definition wildcard_prov := wildcard_prov
-with Definition nil_prov := nil_prov
-with Definition initial_provenance := 0%N
-with Definition provenance_to_prov := fun (pr : Provenance) => Some [pr]
-with Definition access_allowed := fun (pr : Prov) (aid : AllocationId)
-    => match pr with
-       | None => true (* Wildcard can access anything. *)
-       | Some prset =>
-         match aid with
-         | None => true (* Wildcard, can be accessed by anything. *)
-         | Some aid =>
-           existsb (N.eqb aid) prset
-         end
-       end.  
+Module Fin_PTOI_HAS_POINTER_ARITHMETIC <: HAS_POINTER_ARITHMETIC FinAddrType := Fin_HAS_POINTER_ARITHMETIC_CORE  <+ HAS_POINTER_ARITHMETIC_HELPERS FinAddrType.
 
-  Definition Provenance := Provenance.
-  Definition AllocationId := AllocationId.
-  Definition Prov := Prov.
-  Definition wildcard_prov : Prov := wildcard_prov.
-  Definition nil_prov : Prov := nil_prov.
-  Definition address_provenance (a : FinAddr.addr) : Prov
-    := snd a.
-
-  (* Does the provenance set pr allow for access to aid? *)
-  Definition access_allowed (pr : Prov) (aid : AllocationId) : bool
-    := match pr with
-       | None => true (* Wildcard can access anything. *)
-       | Some prset =>
-         match aid with
-         | None => true (* Wildcard, can be accessed by anything. *)
-         | Some aid =>
-           existsb (N.eqb aid) prset
-         end
-       end.
-
-  Definition aid_access_allowed (pr : AllocationId) (aid : AllocationId) : bool
-    := match pr with
-       | None => true
-       | Some pr =>
-         match aid with
-         | None => true
-         | Some aid =>
-           N.eqb pr aid
-         end
-       end.
-
-  Definition allocation_id_to_prov (aid : AllocationId) : Prov
-    := fmap (fun x => [x]) aid.
-
-  Definition provenance_to_allocation_id (pr : Provenance) : AllocationId
-    := Some pr.
-
-  Definition provenance_to_prov (pr : Provenance) : Prov
-    := Some [pr].
-
-  Definition next_provenance (pr : Provenance) : Provenance
-    := N.succ pr.
-
-  Definition initial_provenance : Provenance
-    := 0%N.
-
-  Definition provenance_lt (p1 p2 : Provenance) : Prop
-    := N.lt p1 p2.
-
-  Lemma aid_access_allowed_refl :
-    forall aid, aid_access_allowed aid aid = true.
-  Proof.
-    intros aid.
-    unfold aid_access_allowed.
-    destruct aid; auto.
-    rewrite N.eqb_refl.
-    auto.
-  Qed.
-
-  Lemma access_allowed_refl :
-    forall aid,
-      access_allowed (allocation_id_to_prov aid) aid = true.
-  Proof.
-    intros aid.
-    unfold access_allowed.
-    cbn.
-    destruct aid; auto.
-    cbn.
-    rewrite N.eqb_refl.
-    cbn.
-    auto.
-  Qed.
-
-  Lemma allocation_id_to_prov_inv:
-    forall aid aid',
-      allocation_id_to_prov aid = allocation_id_to_prov aid' ->
-      aid = aid'.
-  Proof.
-    intros aid aid' H.
-    unfold allocation_id_to_prov in *.
-    cbn in *.
-    destruct aid, aid'; inv H; auto.
-  Qed.
-
-  Lemma provenance_to_allocation_id_inv :
-    forall pr pr',
-      provenance_to_allocation_id pr = provenance_to_allocation_id pr' ->
-      pr = pr'.
-  Proof.
-    intros pr pr' H.
-    unfold provenance_to_allocation_id in *.
-    inv H; auto.
-  Qed.
-
-  Lemma allocation_id_to_prov_provenance_to_allocation_id :
-    forall pr,
-      allocation_id_to_prov (provenance_to_allocation_id pr) = provenance_to_prov pr.
-  Proof.
-    intros pr.
-    cbn.
-    auto.
-  Qed.
-
-  Lemma provenance_eq_dec :
-    forall (pr pr' : Provenance),
-      {pr = pr'} + {pr <> pr'}.
-  Proof.
-    unfold Provenance.
-    unfold Provenance.Provenance.
-    intros pr pr'.
-    apply N.eq_dec.
-  Defined.
-
-  Lemma provenance_eq_dec_refl :
-    forall (pr : Provenance),
-      true = provenance_eq_dec pr pr.
-  Proof.
-    intros pr.
-    destruct provenance_eq_dec; cbn; auto.
-    exfalso; auto.
-  Qed.
-
-  Lemma aid_eq_dec :
-    forall (aid aid' : AllocationId),
-      {aid = aid'} + {aid <> aid'}.
-  Proof.
-    intros aid aid'.
-    destruct aid, aid'; auto.
-    pose proof provenance_eq_dec p p0.
-    destruct H; subst; auto.
-    right.
-    intros CONTRA. inv CONTRA; contradiction.
-    right; intros CONTRA; inv CONTRA.
-    right; intros CONTRA; inv CONTRA.
-  Qed.
-
-  Lemma aid_eq_dec_refl :
-    forall (aid : AllocationId),
-      true = aid_eq_dec aid aid.
-  Proof.
-    intros aid.
-    destruct (aid_eq_dec aid aid); cbn; auto.
-    exfalso; auto.
-  Qed.
-
-  #[global] Instance access_allowed_Proper :
-    Proper (eq ==> (fun aid aid' => true = (aid_eq_dec aid aid')) ==> eq) access_allowed.
-  Proof.
-    unfold Proper, respectful.
-    intros x y H x0 y0 H0.
-    subst.
-    unfold access_allowed.
-    symmetry in H0.
-    eapply proj_sumbool_true in H0.
-    subst.
-    reflexivity.
-  Defined.
-
-  #[global] Instance provenance_lt_trans : Transitive provenance_lt.
-  Proof.
-    unfold Transitive.
-    intros x y z XY YZ.
-    unfold provenance_lt in *.
-    lia.
-  Defined.
-
-  Lemma provenance_lt_next_provenance :
-    forall pr,
-      provenance_lt pr (next_provenance pr).
-  Proof.
-    unfold provenance_lt, next_provenance.
-    lia.
-  Qed.
-
-  Lemma provenance_lt_nrefl :
-    forall pr,
-      ~ provenance_lt pr pr.
-  Proof.
-    intros pr.
-    unfold provenance_lt.
-    lia.
-  Qed.
-
-  #[global] Instance provenance_lt_antisym : Antisymmetric Provenance eq provenance_lt.
-  Proof.
-    unfold Antisymmetric.
-    intros x y XY YX.
-    unfold provenance_lt in *.
-    lia.
-  Defined.
-
-  Lemma next_provenance_neq :
-    forall pr,
-      pr <> next_provenance pr.
-  Proof.
-    intros pr.
-    unfold next_provenance.
-    lia.
-  Qed.
-
-  Lemma access_allowed_aid_neq :
-    forall aid1 aid2,
-      aid1 <> aid2 ->
-      access_allowed
-        (allocation_id_to_prov (Some aid1)) (Some aid2) = false.
-  Proof.
-    intros aid1 aid2 NEQ.
-    unfold access_allowed.
-    unfold allocation_id_to_prov.
-    cbn.
-    rewrite orb_false_r.
-    eapply N.eqb_neq.
-    eauto.
-  Qed.
-
-  Lemma access_allowed_aid_eq :
-    forall aid1 aid2,
-      access_allowed
-        (allocation_id_to_prov (Some aid1)) (Some aid2) = true ->
-      aid1 = aid2.
-  Proof.
-    intros aid1 aid2 ACCESS.
-    unfold access_allowed, allocation_id_to_prov in *.
-    cbn in ACCESS.
-    rewrite orb_false_r in ACCESS.
-    eapply N.eqb_eq in ACCESS.
-    auto.
-  Qed.
-
-  (* Debug *)
-  Definition show_prov (pr : Prov) := Show.show pr.
-  Definition show_provenance (pr : Provenance) := Show.show pr.
-  Definition show_allocation_id (aid : AllocationId) := Show.show aid.
-End FinPROV.
-
-Module Type FinPROV <: HAS_PROVENANCE FinAddrType.
-  Definition address_provenance (a : FinAddrType.t) ProvSet.
-End FinPROV.
-
-Module FinAddr <: ADDRESS := FinAddrType <+ FinNull <+ FinPTOI <+ Fin_HAS_POINTER_ARITHMETIC_CORE <+ HAS_POINTER_ARITHMETIC_HELPERS.
-
-
-Module FinITOP : ITOP(FinAddr)(FinPROV)(FinPTOI)
-with Definition int_to_ptr :=
-  fun (i : Z) (pr : Prov) =>
-    if (i <? 0)%Z || (i >=? @Integers.modulus 64)%Z
-    then Oom ("FinITOP.int_to_ptr: out of range (" ++ show i ++ ").")
-    else NoOom (@Integers.repr 64 i, pr).
-
-  Import FinAddr.
-  Import FinPROV.
+Module Fin_PTOI_ARITH_EXTRAS <: PTOI_ARITH_EXTRAS FinAddrType FinPTOI Fin_PTOI_HAS_POINTER_ARITHMETIC.
   Import FinPTOI.
-
-  Definition int_to_ptr (i : Z) (pr : Prov) : OOM addr
-    := if (i <? 0)%Z || (i >=? @Integers.modulus 64)%Z
-       then Oom ("FinITOP.int_to_ptr: out of range (" ++ show i ++ ").")
-       else NoOom (Integers.repr i, pr).
-
-  Lemma int_to_ptr_provenance :
-    forall (x : Z) (p : Prov) (a : addr),
-      int_to_ptr x p = ret a ->
-      FinPROV.address_provenance a = p.
+  Import Fin_PTOI_HAS_POINTER_ARITHMETIC.
+  Lemma ptr_to_int_ptr_add :
+    forall (ptr ptr' : FinAddrType.t) (x : Z),
+      ptr_add ptr x = inr ptr' ->
+      ptr_to_int ptr' = ptr_to_int ptr + x.
   Proof.
-    intros x p a IP.
-    unfold int_to_ptr in *.
-    destruct ((x <? 0)%Z || (x >=? @Integers.modulus 64)); inv IP; auto.
+    intros ptr ptr' x H.
+    unfold ptr_to_int.
+    unfold ptr_add in *.
+    cbn in *.
+    destruct ptr, ptr'; cbn in *.
+    break_match_hyp_inv.
+    rewrite (Integers.unsigned_repr (@Integers.unsigned 64 i + x)); unfold Integers.max_unsigned;
+      lia.
   Qed.
+End Fin_PTOI_ARITH_EXTRAS.
 
+Module Fin_HAS_METADATA <: HAS_METADATA N_ProvSet FinAddrType.
+  Definition extract_metadata (addr : FinAddrType.t) : N_ProvSet.t :=
+    snd addr.
+End Fin_HAS_METADATA.
+
+(* TODO: Move to utility *)
+Module METADATA_PROVENANCE_ID (MD : Typ) <: METADATA_PROVENANCE MD MD.
+  Definition metadata_provenance (md : MD.t) := md.
+End METADATA_PROVENANCE_ID.
+
+Module Fin_HAS_ITOP <: HAS_ITOP N_ProvSet FinAddrType Fin_HAS_METADATA.
+  Definition int_to_ptr :=
+    fun (i : Z) (pr : Prov) =>
+      if (i <? 0)%Z || (i >=? @Integers.modulus 64)%Z
+      then Oom ("FinITOP.int_to_ptr: out of range (" ++ show i ++ ").")
+      else NoOom (@Integers.repr 64 i, pr).
+
+  Lemma int_to_ptr_metadata :
+    forall (x : Z) (p : N_ProvSet.t) (a : FinAddrType.t),
+      int_to_ptr x p = ret a ->
+      Fin_HAS_METADATA.extract_metadata a = p.
+  Proof.
+    intros x p a H.
+    destruct a; cbn in *.
+    unfold int_to_ptr in *.
+    break_match_hyp_inv; auto.
+  Qed.
+End Fin_HAS_ITOP.
+
+Module Fin_PTOI_ITOP_EXTRA <: PTOI_ITOP_EXTRA N_ProvSet FinAddrType Fin_HAS_METADATA Fin_HAS_ITOP FinPTOI.
+  Import FinPTOI Fin_HAS_METADATA Fin_HAS_ITOP.
   Lemma int_to_ptr_ptr_to_int :
-    forall (a : addr) (p : Prov),
-      address_provenance a = p ->
+    forall (a : FinAddrType.t) (p : N_ProvSet.t),
+      extract_metadata a = p ->
       int_to_ptr (ptr_to_int a) p = ret a.
   Proof.
-    intros a p PROV.
-    unfold int_to_ptr.
-    unfold ptr_to_int.
-    destruct a; cbn.
-    pose proof (@Integers.unsigned_range 64 i) as R.
-    destruct ((@Integers.unsigned 64 i <? 0)%Z || (@Integers.unsigned 64 i >=? @Integers.modulus 64)) eqn:RANGE; [lia|].
+    intros a p H.
+    cbn in *.
+    unfold int_to_ptr, ptr_to_int, extract_metadata in *.
+    pose proof (Integers.unsigned_range (fst a)).
+    break_match; try lia.
     rewrite Integers.repr_unsigned.
-    inv PROV; cbn; auto.
+    destruct a; cbn in *; subst; auto.
   Qed.
 
   Lemma int_to_ptr_ptr_to_int_exists :
-    forall (a : addr) (p : Prov),
+    forall (a : FinAddrType.t) (p : N_ProvSet.t),
     exists a',
       int_to_ptr (ptr_to_int a) p = ret a' /\
         ptr_to_int a' = ptr_to_int a /\
-        address_provenance a' = p.
+        extract_metadata a' = p.
   Proof.
-    intros [a prov] p.
-    exists (a, p).
-    split; auto.
-    unfold int_to_ptr, ptr_to_int.
-    cbn in *.
-    destruct ((Integers.unsigned a <? 0)%Z || (Integers.unsigned a >=? Integers.modulus)) eqn:BOUNDS.
-    - (* Out of bounds *)
-      exfalso.
-      destruct a.
-      cbn in *.
-      lia.
-    - rewrite Integers.repr_unsigned.
-      reflexivity.
+    intros a p.
+    destruct a.
+    exists (i, p).
+    unfold int_to_ptr, ptr_to_int, extract_metadata in *.
+    pose proof (Integers.unsigned_range i); cbn in *.
+    break_match; try lia.
+    rewrite Integers.repr_unsigned.
+    cbn; auto.
   Qed.
 
   Lemma ptr_to_int_int_to_ptr :
-    forall (x : Z) (p : Prov) (a : addr),
+    forall (x : Z) (p : N_ProvSet.t) (a : FinAddrType.t),
       int_to_ptr x p = ret a ->
       ptr_to_int a = x.
   Proof.
-    intros x p a IP.
-    unfold int_to_ptr in *.
-    destruct ((x <? 0)%Z || (x >=? @Integers.modulus 64)) eqn:RANGE; inv IP; auto.
-    unfold ptr_to_int, fst.
-    rewrite (@Integers.unsigned_repr 64); auto.
-    unfold Integers.max_unsigned.
-    lia.
+    intros x p a H.
+    unfold int_to_ptr, ptr_to_int, extract_metadata in *.
+    break_match_hyp_inv.
+    cbn.
+    rewrite Integers.unsigned_repr; auto.
+    unfold Integers.max_unsigned; lia.
   Qed.
-End FinITOP.
+End Fin_PTOI_ITOP_EXTRA.
+
+Module FinAddr <: ADDRESS N_ProvSet N_ProvSet := FinAddrType <+ FinNull <+ FinPTOI <+ Fin_PTOI_HAS_POINTER_ARITHMETIC <+ Fin_PTOI_ARITH_EXTRAS <+ METADATA_PROVENANCE_ID N_ProvSet <+ Fin_HAS_METADATA <+ HAS_PROVENANCE N_ProvSet N_ProvSet <+ Fin_HAS_ITOP <+ Fin_PTOI_ITOP_EXTRA.
