src/mem/Addresses/TypeModules.v
@@ -1,0 +1,24 @@
+From Coq Require Import
+  Structures.Equalities.
+
+Module UNIT_TYP <: DecidableType.
+  Definition t := unit.
+  Definition eq : unit -> unit -> Prop := Logic.eq.
+
+  Lemma eq_dec : forall (a b : unit), {a = b} + {a <> b}.
+  Proof.
+    intros [] []; auto.
+  Qed.
+
+  #[global] Instance eq_equiv : Equivalence eq.
+  typeclasses eauto.
+  Defined.
+End UNIT_TYP.
+
+Module Type HasDefault (Import T : Typ).
+  Parameter default : t.
+End HasDefault.
+
+Module UNIT_HAS_DEFAULT <: HasDefault UNIT_TYP.
+  Definition default := tt.
+End UNIT_HAS_DEFAULT.
